theories/input_lang/interp.v
@@ -1,6 +1,8 @@
-From Equations Require Import Equations.
-From gitrees Require Import gitree.
+From gitrees Require Import gitree lang_generic.
 From gitrees.input_lang Require Import lang.
+
+Require Import Binding.Lib.
+Require Import Binding.Set.
 
 Notation stateO := (leibnizO state).
 
@@ -18,69 +20,29 @@ Program Definition outputE : opInterp :=
 
 Definition ioE := @[inputE;outputE].
 
-Definition wrap_reifier X `{Cofe X} (A B : ofe) :
-  (A * stateO -n> option (B * stateO))%type ->
-  (A * stateO * (B -n> laterO X) → option (laterO X * stateO))%type :=
-  λ f,
-    λ x, let '(i, σ, k)  := x in
-         fmap (prodO_map k idfun) (f (i, σ)).
-#[export] Instance wrap_reifier_ne X `{Cofe X} (A B : ofe) f :
-  NonExpansive (wrap_reifier X A B f).
-Proof.
-  intros n [[a1 σ1] k1] [[a2 σ2] k2] [[Ha Hσ] Hk]. simpl.
-  solve_proper.
-Qed.
-
 (* INPUT *)
-Definition reify_input' X `{Cofe X} : unitO * stateO →
+Definition reify_input X `{Cofe X} : unitO * stateO →
                                       option (natO * stateO) :=
     λ '(o, σ), Some (update_input σ : prodO natO stateO).
-#[export] Instance reify_input'_ne X `{Cofe X} :
-  NonExpansive (reify_input' X).
+#[export] Instance reify_input_ne X `{Cofe X} :
+  NonExpansive (reify_input X).
 Proof.
   intros ?[[]][[]][_?]. simpl in *. f_equiv.
   repeat f_equiv. done.
 Qed.
 
-Definition reify_input X `{Cofe X} : unitO * stateO * (natO -n> laterO X) →
-                                     option (laterO X * stateO) :=
-  λ '(o, σ, k), fmap (prodO_map k idfun) (reify_input' X (o, σ)).
-#[export] Instance reify_input_ne X `{Cofe X} :
-  NonExpansive (reify_input X : prodO (prodO unitO stateO)
-                                  (natO -n> laterO X) →
-                                  optionO (prodO (laterO X) stateO)).
-Proof.
-  intros n [[? σ1] k1] [[? σ2] k2]. simpl.
-  intros [[_ ->] Hk]. simpl in *.
-  repeat f_equiv. assumption.
-Qed.
-
 (* OUTPUT *)
-Definition reify_output' X `{Cofe X} : (natO * stateO) →
+Definition reify_output X `{Cofe X} : (natO * stateO) →
                                        option (unitO * stateO) :=
   λ '(n, σ), Some((), update_output n σ : stateO).
-#[export] Instance reify_output'_ne X `{Cofe X} :
-  NonExpansive (reify_output' X).
+#[export] Instance reify_output_ne X `{Cofe X} :
+  NonExpansive (reify_output X).
 Proof.
   intros ?[][][]. simpl in *.
   repeat f_equiv; done.
 Qed.
 
-
-Definition reify_output X `{Cofe X} : (natO * stateO * (unitO -n> laterO X)) →
-                                      optionO (prodO (laterO X) stateO) :=
-  λ '(n, σ, k), fmap (prodO_map k idfun)
-                     (reify_output' X (n, σ)).
-#[export] Instance reify_output_ne X `{Cofe X} :
-  NonExpansive (reify_output X : prodO (prodO natO stateO)
-                                   (unitO -n> laterO X) →
-                                 optionO (prodO (laterO X) stateO)).
-Proof.
-  intros ? [[]] [[]] []; simpl in *.
-  repeat f_equiv; first assumption; apply H0.
-Qed.
-
-Canonical Structure reify_io : sReifier.
+Canonical Structure reify_io : sReifier NotCtxDep.
 Proof.
   simple refine {| sReifier_ops := ioE;
                    sReifier_state := stateO
@@ -97,15 +59,6 @@ Section constructors.
   Context {subOfe0 : SubOfe natO A}.
   Notation IT := (IT E A).
   Notation ITV := (ITV E A).
-
-  Global Instance ioEctx_indep :
-    ∀ (o : opid ioE), CtxIndep reify_io IT o.
-  Proof.
-    intros op.
-    destruct op as [[] | [ | []]].
-    - constructor. by exists (OfeMor (reify_input' IT)).
-    - constructor. by exists (OfeMor (reify_output' IT)).
-  Qed.
 
   Program Definition INPUT : (nat -n> IT) -n> IT := λne k, Vis (E:=E) (subEff_opid (inl ()))
                                                              (subEff_ins (F:=ioE) (op:=(inl ())) ())
@@ -137,9 +90,9 @@ End constructors.
 
 Section weakestpre.
   Context {sz : nat}.
-  Variable (rs : gReifiers sz).
+  Variable (rs : gReifiers NotCtxDep sz).
   Context {subR : subReifier reify_io rs}.
-  Notation F := (gReifiers_ops rs).
+  Notation F := (gReifiers_ops NotCtxDep rs).
   Context {R} `{!Cofe R}.
   Context `{!SubOfe natO R}.
   Notation IT := (IT F R).
@@ -155,7 +108,7 @@ Section weakestpre.
   Proof.
     intros Hs. iIntros "Hs Ha".
     unfold INPUT. simpl.
-    iApply (wp_subreify with "Hs").
+    iApply (wp_subreify_ctx_indep with "Hs").
     { simpl. rewrite Hs//=. }
     { simpl. by rewrite ofe_iso_21. }
     iModIntro. done.
@@ -169,7 +122,7 @@ Section weakestpre.
   Proof.
     intros Hs. iIntros "Hs Ha".
     unfold OUTPUT. simpl.
-    iApply (wp_subreify rs with "Hs").
+    iApply (wp_subreify_ctx_indep rs with "Hs").
     { simpl. by rewrite Hs. }
     { simpl. done. }
     iModIntro. iIntros "H1 H2".
@@ -180,13 +133,19 @@ End weakestpre.
 
 Section interp.
   Context {sz : nat}.
-  Variable (rs : gReifiers sz).
+  Variable (rs : gReifiers NotCtxDep sz).
   Context {subR : subReifier reify_io rs}.
-  Context {R} `{!Cofe R}.
+  Context {R} `{CR : !Cofe R}.
   Context `{!SubOfe natO R}.
-  Notation F := (gReifiers_ops rs).
+  Notation F := (gReifiers_ops NotCtxDep rs).
   Notation IT := (IT F R).
   Notation ITV := (ITV F R).
+
+  Global Instance denot_cont_ne (κ : IT -n> IT) :
+    NonExpansive (λ x : IT, Tau (laterO_map κ (Next x))).
+  Proof.
+    solve_proper.
+  Qed.
 
   (** Interpreting individual operators *)
   Program Definition interp_input {A} : A -n> IT :=
@@ -205,18 +164,49 @@ Section interp.
   Typeclasses Opaque interp_natop.
 
   Opaque laterO_map.
-  Program Definition interp_rec_pre {A} (body : prodO IT (prodO IT A) -n> IT)
-    : laterO (A -n> IT) -n> A -n> IT :=
-    λne self env, Fun $ laterO_map (λne (self : A -n> IT) (a : IT),
-                                     body (self env,(a,env))) self.
-  Solve All Obligations with first [ solve_proper | solve_proper_please ].
+  Program Definition interp_rec_pre {S : Set} (body : @interp_scope F R _ (inc (inc S)) -n> IT)
+    : laterO (@interp_scope F R _ S -n> IT) -n> @interp_scope F R _ S -n> IT :=
+    λne self env, Fun $ laterO_map (λne (self : @interp_scope F R  _ S -n> IT) (a : IT),
+                      body (@extend_scope F R _ _ (@extend_scope F R _ _ env (self env)) a)) self.
+  Next Obligation.
+    intros.
+    solve_proper_prepare.
+    f_equiv; intros [| [| y']]; simpl; solve_proper.
+  Qed.
+  Next Obligation.
+    intros.
+    solve_proper_prepare.
+    f_equiv; intros [| [| y']]; simpl; solve_proper.
+  Qed.
+  Next Obligation.
+    intros.
+    solve_proper_prepare.
+    do 3 f_equiv; intros ??; simpl; f_equiv;
+    intros [| [| y']]; simpl; solve_proper.
+  Qed.
+  Next Obligation.
+    intros.
+    solve_proper_prepare.
+    by do 2 f_equiv.
+  Qed.
 
-  Definition interp_rec {A} body : A -n> IT := mmuu (interp_rec_pre body).
-  Program Definition ir_unf {A} (body : prodO IT (prodO IT A) -n> IT) env : IT -n> IT :=
-    λne a, body (interp_rec body env, (a,env)).
-  Solve All Obligations with first [ solve_proper | solve_proper_please ].
+  Program Definition interp_rec {S : Set}
+    (body : @interp_scope F R _ (inc (inc S)) -n> IT) :
+    @interp_scope F R _ S -n> IT :=
+    mmuu (interp_rec_pre body).
 
-  Lemma interp_rec_unfold {A} (body : prodO IT (prodO IT A) -n> IT) env :
+  Program Definition ir_unf {S : Set}
+    (body : @interp_scope F R _ (inc (inc S)) -n> IT) env : IT -n> IT :=
+    λne a, body (@extend_scope F R _ _
+                   (@extend_scope F R _ _ env (interp_rec body env))
+                   a).
+  Next Obligation.
+    intros.
+    solve_proper_prepare.
+    f_equiv. intros [| [| y']]; simpl; solve_proper.
+  Qed.
+
+  Lemma interp_rec_unfold {S : Set} (body : @interp_scope F R _ (inc (inc S)) -n> IT) env :
     interp_rec body env ≡ Fun $ Next $ ir_unf body env.
   Proof.
     trans (interp_rec_pre body (Next (interp_rec body)) env).
@@ -242,412 +232,458 @@ Section interp.
   Program Definition interp_nat (n : nat) {A} : A -n> IT :=
     λne env, Ret n.
 
-  Program Definition interp_cont {A} (K : A -n> (IT -n> IT)) : A -n> IT := λne env, Fun (Next (K env)).
-  Next Obligation.
-    solve_proper.
-  Qed.
+  Program Definition interp_applk {A}
+    (K : A -n> (IT -n> IT))
+    (q : A -n> IT)
+    : A -n> (IT -n> IT) :=
+    λne env t, interp_app (λne env, K env t) q env.
+  Solve All Obligations with solve_proper.
 
-  Program Definition interp_applk {A} (q : A -n> IT) (K : A -n> (IT -n> IT)) : A -n> (IT -n> IT) := λne env t, interp_app q (λne env, K env t) env.
-  Next Obligation.
-    solve_proper.
-  Qed.
-  Next Obligation.
-    solve_proper.
-  Qed.
-  Next Obligation.
-    solve_proper.
-  Qed.
+  Program Definition interp_apprk {A}
+    (q : A -n> IT)
+    (K : A -n> (IT -n> IT))
+    : A -n> (IT -n> IT) :=
+    λne env t, interp_app q (λne env, K env t) env.
+  Solve All Obligations with solve_proper.
 
-  Program Definition interp_apprk {A} (K : A -n> (IT -n> IT)) (q : A -n> IT) : A -n> (IT -n> IT) := λne env t, interp_app (λne env, K env t) q env.
-  Next Obligation.
-    solve_proper.
-  Qed.
-  Next Obligation.
-    solve_proper.
-  Qed.
-  Next Obligation.
-    solve_proper.
-  Qed.
+  Program Definition interp_natoprk {A} (op : nat_op)
+    (q : A -n> IT)
+    (K : A -n> (IT -n> IT)) : A -n> (IT -n> IT) :=
+    λne env t, interp_natop op q (λne env, K env t) env.
+  Solve All Obligations with solve_proper.
+
+  Program Definition interp_natoplk {A} (op : nat_op)
+    (K : A -n> (IT -n> IT))
+    (q : A -n> IT) : A -n> (IT -n> IT) :=
+    λne env t, interp_natop op (λne env, K env t) q env.
+  Solve All Obligations with solve_proper.
+
+  Program Definition interp_ifk {A} (K : A -n> (IT -n> IT)) (q : A -n> IT)
+    (p : A -n> IT) : A -n> (IT -n> IT) :=
+    λne env t, interp_if (λne env, K env t) q p env.
+  Solve All Obligations with solve_proper.
+
+  Program Definition interp_outputk {A} (K : A -n> (IT -n> IT)) :
+    A -n> (IT -n> IT) :=
+    λne env t, interp_output (λne env, K env t) env.
+  Solve All Obligations with solve_proper.
 
   (** Interpretation for all the syntactic categories: values, expressions, contexts *)
   Fixpoint interp_val {S} (v : val S) : interp_scope S -n> IT :=
     match v with
-    | Lit n => interp_nat n
+    | LitV n => interp_nat n
     | RecV e => interp_rec (interp_expr e)
     end
   with interp_expr {S} (e : expr S) : interp_scope S -n> IT :=
-    match e with
-    | Val v => interp_val v
-    | Var x => interp_var x
-    | Rec e => interp_rec (interp_expr e)
-    | App e1 e2 => interp_app (interp_expr e1) (interp_expr e2)
-    | NatOp op e1 e2 => interp_natop op (interp_expr e1) (interp_expr e2)
-    | If e e1 e2 => interp_if (interp_expr e) (interp_expr e1) (interp_expr e2)
-    | Input => interp_input
-    | Output e => interp_output (interp_expr e)
-    end.
-
-  Program Definition interp_ctx_item {S : scope} (K : ectx_item S) : interp_scope S -n> IT -n> IT :=
-    match K with
-    | AppLCtx v2 => λne env t, interp_app (constO t) (interp_val v2) env
-    | AppRCtx e1 => λne env t, interp_app (interp_expr e1) (constO t) env
-    | NatOpLCtx op v2 => λne env t, interp_natop op (constO t) (interp_val v2) env
-    | NatOpRCtx op e1 => λne env t, interp_natop op (interp_expr e1) (constO t) env
-    | IfCtx e1 e2 => λne env t, interp_if (constO t) (interp_expr e1) (interp_expr e2) env
-    | OutputCtx => λne env t, interp_output (constO t) env
-    end.
+         match e with
+         | Val v => interp_val v
+         | Var x => interp_var x
+         | App e1 e2 => interp_app (interp_expr e1) (interp_expr e2)
+         | NatOp op e1 e2 => interp_natop op (interp_expr e1) (interp_expr e2)
+         | If e e1 e2 => interp_if (interp_expr e) (interp_expr e1) (interp_expr e2)
+         | Input => interp_input
+         | Output e => interp_output (interp_expr e)
+         end
+  with interp_ectx {S} (K : ectx S) : interp_scope S -n> (IT -n> IT) :=
+         match K with
+         | EmptyK => λne env, idfun
+         | AppRK e1 K => interp_apprk (interp_expr e1) (interp_ectx K)
+         | AppLK K v2 => interp_applk (interp_ectx K) (interp_val v2)
+         | NatOpRK op e1 K => interp_natoprk op (interp_expr e1) (interp_ectx K)
+         | NatOpLK op K v2 => interp_natoplk op (interp_ectx K) (interp_val v2)
+         | IfK K e1 e2 => interp_ifk (interp_ectx K) (interp_expr e1) (interp_expr e2)
+         | OutputK K => interp_outputk (interp_ectx K)
+         end.
   Solve All Obligations with first [ solve_proper | solve_proper_please ].
 
-  #[global] Instance interp_val_asval {S} (v : val S) D : AsVal (interp_val v D).
+  Global Instance interp_val_asval {S} {D : interp_scope S} (v : val S)
+    : AsVal (interp_val v D).
   Proof.
-    destruct v; simpl; first apply _.
-    rewrite interp_rec_unfold. apply _.
-  Qed.
-  Program Fixpoint interp_ectx {S} (K : ectx S) : interp_scope S -n> IT -n> IT
-    :=
-      match K with
-      | [] => λne env, idfun
-      | Ki::K => λne env, interp_ectx K env ◎ interp_ctx_item Ki env
-      end.
-  Next Obligation. solve_proper. Defined. (* XXX why can't i qed here? *)
-
-  Lemma interp_ctx_item_fill {S} (Ki : ectx_item S) e env :
-    interp_expr (fill_item Ki e) env ≡ interp_ctx_item Ki env (interp_expr e env).
-  Proof. destruct Ki; reflexivity. Qed.
-
-  Lemma interp_ectx_fill {S} (K : ectx S) e env :
-    interp_expr (fill K e) env ≡ interp_ectx K env (interp_expr e env).
-  Proof.
-    revert e; induction K as [|Ki K]=>e; first done.
-    rewrite IHK. simpl. rewrite interp_ctx_item_fill. done.
+    destruct v; simpl.
+    - apply _.
+    - rewrite interp_rec_unfold. apply _.
   Qed.
 
-  (** Applying renamings and subsitutions to the interpretation of scopes *)
-  Equations interp_rens_scope {S S' : scope}
-            (E : interp_scope (E:=F) (R:=R) S') (s : rens S S') : interp_scope (E:=F) (R:=R) S :=
-    interp_rens_scope (S:=[]) E s := tt : interp_scope [];
-    interp_rens_scope (S:=_::_) E s :=
-      (interp_var (hd_ren s) E, interp_rens_scope E (tl_ren s)).
+  Global Instance ArrEquiv {A B : Set} : Equiv (A [→] B) :=
+    fun f g => ∀ x, f x = g x.
 
-  Equations interp_subs_scope {S S' : scope}
-            (E : interp_scope (E:=F) (R:=R) S') (s : subs S S') : interp_scope (E:=F) (R:=R) S :=
-    interp_subs_scope (S:=[]) E s := tt : interp_scope [];
-    interp_subs_scope (S:=_::_) E s :=
-      (interp_expr (hd_sub s) E, interp_subs_scope E (tl_sub s)).
+  Global Instance ArrDist {A B : Set} `{Dist B} : Dist (A [→] B) :=
+    fun n => fun f g => ∀ x, f x ≡{n}≡ g x.
 
-
-  Global Instance interp_rens_scope_ne S S2 n :
-    Proper ((dist n) ==> (≡) ==> (dist n)) (@interp_rens_scope S S2).
+  Global Instance ren_scope_proper {S S'} :
+    Proper ((≡) ==> (≡) ==> (≡)) (@ren_scope F _ CR S S').
   Proof.
     intros D D' HE s1 s2 Hs.
-    induction S as [|τ' S]; simp interp_rens_scope; auto.
+    intros x; simpl.
     f_equiv.
-    - unfold hd_ren; rewrite Hs. by f_equiv.
-    - apply IHS. intros v. unfold tl_ren; by rewrite Hs.
-  Qed.
-  Global Instance interp_subs_scope_ne S S2 n :
-    Proper ((dist n) ==> (≡) ==> (dist n)) (@interp_subs_scope S S2).
-  Proof.
-    intros D D' HE s1 s2 Hs.
-    induction S as [|τ' S]; simp interp_subs_scope; auto.
-    f_equiv.
-    - unfold hd_sub; by rewrite Hs HE.
-    - apply IHS. intros v. unfold tl_sub; by rewrite Hs.
-  Qed.
-  Global Instance interp_rens_scope_proper S S2 :
-    Proper ((≡) ==> (≡) ==> (≡)) (@interp_rens_scope S S2).
-  Proof.
-    intros D D' HE s1 s2 Hs.
-    induction S as [|τ' S]; simp interp_rens_scope; auto.
-    f_equiv.
-    - unfold hd_ren; rewrite Hs.
-      by rewrite HE.
-    - apply IHS. intros v. unfold tl_ren; by rewrite Hs.
-  Qed.
-  Global Instance interp_subs_scope_proper S S2 :
-    Proper ((≡) ==> (≡) ==> (≡)) (@interp_subs_scope S S2).
-  Proof.
-    intros D D' HE s1 s2 Hs.
-    induction S as [|τ' S]; simp interp_subs_scope; auto.
-    f_equiv.
-    - unfold hd_sub; by rewrite Hs HE.
-    - apply IHS. intros v. unfold tl_sub; by rewrite Hs.
-  Qed.
+    - apply Hs.
+    - apply HE.
+ Qed.
 
-  (** ** The substituion lemma, for renamings and substitutions *)
-  Lemma interp_rens_scope_tl_ren {S S2} x D (r : rens S S2) :
-    interp_rens_scope ((x, D) : interp_scope (()::S2)) (tl_ren (rens_lift r))
-                    ≡ interp_rens_scope D r.
+  Lemma interp_expr_ren {S S'} env
+    (δ : S [→] S') (e : expr S) :
+    interp_expr (fmap δ e) env ≡ interp_expr e (ren_scope δ env)
+  with interp_val_ren {S S'} env
+         (δ : S [→] S') (e : val S) :
+    interp_val (fmap δ e) env ≡ interp_val e (ren_scope δ env)
+  with interp_ectx_ren {S S'} env
+         (δ : S [→] S') (e : ectx S) :
+    interp_ectx (fmap δ e) env ≡ interp_ectx e (ren_scope δ env).
   Proof.
-    induction S as [|τ' S]; simp interp_rens_scope; eauto.
-    f_equiv.
-    { unfold hd_ren, tl_ren. simp rens_lift interp_var.
-      done. }
-    { rewrite -IHS. f_equiv. clear.
-      intros v. dependent elimination v;
-        unfold hd_ren, tl_ren; simp rens_lift; auto. }
-  Qed.
-
-  Lemma interp_rens_scope_idren {S} (D : interp_scope S) :
-    interp_rens_scope D (@idren S) ≡ D.
-  Proof.
-    induction S as [|[] S]; simp interp_rens_scope.
-    { by destruct D. }
-    destruct D as [x D]. simp interp_var. simpl.
-    f_equiv.
-    trans (interp_rens_scope ((x, D) : interp_scope (()::S)) (tl_ren (rens_lift idren))).
-    { f_equiv. intros v. unfold tl_ren.
-      reflexivity. }
-    rewrite interp_rens_scope_tl_ren.
-    apply IHS.
-  Qed.
-
-  Lemma interp_expr_ren {S D : scope} (M : expr S) (r : rens S D) :
-    ∀ (E : interp_scope D),
-      interp_expr (ren_expr M r) E ≡ interp_expr M (interp_rens_scope E r)
-  with interp_val_ren {S D : scope} (v : val S) (r : rens S D) :
-    ∀ (E : interp_scope D),
-      interp_val (ren_val v r) E ≡ interp_val v (interp_rens_scope E r).
-  Proof.
-    - revert D r. induction M=> D r D2; simpl; simp ren_expr.
-      all: try by (simpl; repeat intro; simpl; repeat f_equiv; eauto).
-      + (* variable *) revert r.
-        induction v=>r.
-        * simp interp_var interp_rens_scope. done.
-        * simp interp_var interp_rens_scope. simpl.
-          apply (IHv (tl_ren r)).
-      + (* recursive functions *) simp ren_expr. simpl.
+    - destruct e; simpl.
+      + by apply interp_val_ren.
+      + reflexivity.
+      + repeat f_equiv; by apply interp_expr_ren.
+      + repeat f_equiv; by apply interp_expr_ren.
+      + repeat f_equiv; by apply interp_expr_ren.
+      + repeat f_equiv; by apply interp_expr_ren.
+      + repeat f_equiv; by apply interp_expr_ren.
+    - destruct e; simpl.
+      + reflexivity.
+      + clear -interp_expr_ren.
         apply bi.siProp.internal_eq_soundness.
         iLöb as "IH".
         rewrite {2}interp_rec_unfold.
-        rewrite {2}(interp_rec_unfold (interp_expr M)).
-        iApply f_equivI. iNext. iApply internal_eq_pointwise.
+        rewrite {2}(interp_rec_unfold (interp_expr e)).
+        do 1 iApply f_equivI. iNext.
+        iApply internal_eq_pointwise.
         rewrite /ir_unf. iIntros (x). simpl.
         rewrite interp_expr_ren.
         iApply f_equivI.
-        simp interp_rens_scope interp_var. simpl.
-        rewrite !interp_rens_scope_tl_ren.
-        iRewrite "IH".
-        done.
-    - revert D r. induction v=> D r D2; simpl; simp ren_val; eauto.
-      (* recursive functions *)
-      simp ren_expr. simpl.
-      apply bi.siProp.internal_eq_soundness.
-      iLöb as "IH".
-      rewrite {2}interp_rec_unfold.
-      rewrite {2}(interp_rec_unfold (interp_expr e)).
-      iApply f_equivI. iNext. iApply internal_eq_pointwise.
-      rewrite /ir_unf. iIntros (x). simpl.
-      rewrite interp_expr_ren.
-      iApply f_equivI.
-      simp interp_rens_scope interp_var. simpl.
-      rewrite !interp_rens_scope_tl_ren.
-      iRewrite "IH".
-      done.
+        iApply internal_eq_pointwise.
+        iIntros (y').
+        destruct y' as [| [| y]]; simpl; first done.
+        * by iRewrite - "IH".
+        * done.
+    - destruct e; simpl; intros ?; simpl.
+      + reflexivity.
+      + repeat f_equiv; by apply interp_ectx_ren.
+      + repeat f_equiv; [by apply interp_ectx_ren | by apply interp_expr_ren | by apply interp_expr_ren].
+      + repeat f_equiv; [by apply interp_ectx_ren | by apply interp_val_ren].
+      + repeat f_equiv; [by apply interp_expr_ren | by apply interp_ectx_ren].
+      + repeat f_equiv; [by apply interp_expr_ren | by apply interp_ectx_ren].
+      + repeat f_equiv; [by apply interp_ectx_ren | by apply interp_val_ren].
   Qed.
 
-  Lemma interp_subs_scope_tl_sub {S S2} x D (s : subs S S2) :
-    interp_subs_scope ((x, D) : interp_scope (()::S2)) (tl_sub (subs_lift s))
-                    ≡ interp_subs_scope D s.
+  Lemma interp_comp {S} (e : expr S) (env : interp_scope S) (K : ectx S):
+    interp_expr (fill K e) env ≡ (interp_ectx K) env ((interp_expr e) env).
   Proof.
-    induction S as [|[] S]; simp interp_subs_scope; first done.
+    revert env.
+    induction K; simpl; intros env; first reflexivity; try (by rewrite IHK).
+    - repeat f_equiv.
+      by rewrite IHK.
+    - repeat f_equiv.
+      by rewrite IHK.
+    - repeat f_equiv.
+      by rewrite IHK.
+  Qed.
+
+  Program Definition sub_scope {S S'} (δ : S [⇒] S') (env : interp_scope S')
+    : interp_scope S := λne x, interp_expr (δ x) env.
+
+  Global Instance SubEquiv {A B : Set} : Equiv (A [⇒] B) := fun f g => ∀ x, f x = g x.
+
+  Global Instance sub_scope_proper {S S'} :
+    Proper ((≡) ==> (≡) ==> (≡)) (@sub_scope S S').
+  Proof.
+    intros D D' HE s1 s2 Hs.
+    intros x; simpl.
     f_equiv.
-    { unfold hd_sub, tl_sub. simp subs_lift interp_var.
-      unfold expr_lift. rewrite interp_expr_ren. f_equiv.
-      trans (interp_rens_scope ((x, D) : interp_scope (()::S2)) (tl_ren (rens_lift idren))).
-      { f_equiv. intros v. unfold tl_ren.
-        simp rens_lift idren. done. }
-      rewrite interp_rens_scope_tl_ren.
-      apply interp_rens_scope_idren. }
-    { rewrite -IHS. f_equiv. clear.
-      intros v. dependent elimination v;
-        unfold hd_sub, tl_sub; simp subs_lift; auto. }
-  Qed.
+    - f_equiv.
+      apply HE.
+    - apply Hs.
+ Qed.
 
-  Lemma interp_subs_scope_idsub {S} (env : interp_scope S) :
-    interp_subs_scope env idsub ≡ env.
+  Lemma interp_expr_subst {S S'} (env : interp_scope S')
+    (δ : S [⇒] S') e :
+    interp_expr (bind δ e) env ≡ interp_expr e (sub_scope δ env)
+  with interp_val_subst {S S'} (env : interp_scope S')
+         (δ : S [⇒] S') e :
+    interp_val (bind δ e) env ≡ interp_val e (sub_scope δ env)
+  with interp_ectx_subst {S S'} (env : interp_scope S')
+         (δ : S [⇒] S') e :
+    interp_ectx (bind δ e) env ≡ interp_ectx e (sub_scope δ env).
   Proof.
-    induction S as [|[] S]; simp interp_subs_scope.
-    { by destruct env. }
-    destruct env as [x env].
-    unfold hd_sub, idsub. simpl.
-    simp interp_var. simpl. f_equiv.
-    etrans; last first.
-    { apply IHS. }
-    rewrite -(interp_subs_scope_tl_sub x env idsub).
-    repeat f_equiv. intro v. unfold tl_sub, idsub; simpl.
-    simp subs_lift. unfold expr_lift. simp ren_expr. done.
-  Qed.
-
-  Lemma interp_expr_subst {S D : scope} (M : expr S) (s : subs S D) :
-    ∀ (E : interp_scope D),
-      interp_expr (subst_expr M s) E ≡ interp_expr M (interp_subs_scope E s)
-  with interp_val_subst {S D : scope} (v : val S) (s : subs S D) :
-    ∀ (E : interp_scope D),
-      interp_val (subst_val v s) E ≡ interp_val v (interp_subs_scope E s).
-  Proof.
-    - revert D s. induction M=> D r D2; simpl; simp subst_expr.
-      all: try by (simpl; repeat intro; simpl; repeat f_equiv; eauto).
-      + (* variable *) revert r.
-        induction v=>r.
-        * simp interp_var interp_rens_scope. done.
-        * simp interp_var interp_rens_scope. simpl.
-          apply (IHv (tl_sub r)).
-      + (* recursive functions *) simpl.
+    - destruct e; simpl.
+      + by apply interp_val_subst.
+      + term_simpl.
+        reflexivity.
+      + repeat f_equiv; by apply interp_expr_subst.
+      + repeat f_equiv; by apply interp_expr_subst.
+      + repeat f_equiv; by apply interp_expr_subst.
+      + f_equiv.
+      + repeat f_equiv; by apply interp_expr_subst.
+    - destruct e; simpl.
+      + reflexivity.
+      + clear -interp_expr_subst.
         apply bi.siProp.internal_eq_soundness.
         iLöb as "IH".
         rewrite {2}interp_rec_unfold.
-        rewrite {2}(interp_rec_unfold (interp_expr M)).
-        iApply f_equivI. iNext. iApply internal_eq_pointwise.
+        rewrite {2}(interp_rec_unfold (interp_expr e)).
+        do 1 iApply f_equivI. iNext.
+        iApply internal_eq_pointwise.
         rewrite /ir_unf. iIntros (x). simpl.
         rewrite interp_expr_subst.
         iApply f_equivI.
-        simp interp_subs_scope interp_var. simpl.
-        rewrite !interp_subs_scope_tl_sub.
-        iRewrite "IH".
-        done.
-    - revert D s. induction v=> D r D2; simpl; simp subst_val; eauto.
-      (* recursive functions *)
-      simp subst_expr. simpl.
-      apply bi.siProp.internal_eq_soundness.
-      iLöb as "IH".
-      rewrite {2}interp_rec_unfold.
-      rewrite {2}(interp_rec_unfold (interp_expr e)).
-      iApply f_equivI. iNext. iApply internal_eq_pointwise.
-      rewrite /ir_unf. iIntros (x). simpl.
-      rewrite interp_expr_subst.
-      iApply f_equivI.
-      simp interp_subs_scope interp_var. simpl.
-      rewrite !interp_subs_scope_tl_sub.
-      iRewrite "IH".
-      done.
+        iApply internal_eq_pointwise.
+        iIntros (y').
+        destruct y' as [| [| y]]; simpl; first done.
+        * by iRewrite - "IH".
+        * do 2 rewrite interp_expr_ren.
+          iApply f_equivI.
+          iApply internal_eq_pointwise.
+          iIntros (z).
+          done.
+    - destruct e; simpl; intros ?; simpl.
+      + reflexivity.
+      + repeat f_equiv; by apply interp_ectx_subst.
+      + repeat f_equiv; [by apply interp_ectx_subst | by apply interp_expr_subst | by apply interp_expr_subst].
+      + repeat f_equiv; [by apply interp_ectx_subst | by apply interp_val_subst].
+      + repeat f_equiv; [by apply interp_expr_subst | by apply interp_ectx_subst].
+      + repeat f_equiv; [by apply interp_expr_subst | by apply interp_ectx_subst].
+      + repeat f_equiv; [by apply interp_ectx_subst | by apply interp_val_subst].
   Qed.
 
-  (** ** Interpretation is a homomorphism *)
-  #[global] Instance interp_ectx_item_hom {S} (Ki : ectx_item S) env :
-    IT_hom (interp_ctx_item Ki env).
-  Proof. destruct Ki; simpl; apply _. Qed.
-  #[global] Instance interp_ectx_hom {S} (K : ectx S) env :
+  (** ** Interpretation is a homomorphism (for some constructors) *)
+
+  #[global] Instance interp_ectx_hom_emp {S} env :
+    IT_hom (interp_ectx (EmptyK : ectx S) env).
+  Proof.
+    simple refine (IT_HOM _ _ _ _ _); intros; auto.
+    simpl. fold (@idfun IT). f_equiv. intro. simpl.
+    by rewrite laterO_map_id.
+  Qed.
+
+  #[global] Instance interp_ectx_hom_output {S} (K : ectx S) env :
+    IT_hom (interp_ectx K env) ->
+    IT_hom (interp_ectx (OutputK K) env).
+  Proof.
+    intros. simple refine (IT_HOM _ _ _ _ _); intros; simpl.
+    - by rewrite !hom_tick.
+    - rewrite !hom_vis.
+      f_equiv. intro. simpl. rewrite -laterO_map_compose.
+      do 2 f_equiv. by intro.
+    - by rewrite !hom_err.
+  Qed.
+
+  #[global] Instance interp_ectx_hom_if {S}
+    (K : ectx S) (e1 e2 : expr S) env :
+    IT_hom (interp_ectx K env) ->
+    IT_hom (interp_ectx (IfK K e1 e2) env).
+  Proof.
+    intros. simple refine (IT_HOM _ _ _ _ _); intros; simpl.
+    - rewrite -IF_Tick. do 3 f_equiv. apply hom_tick.
+    - assert ((interp_ectx K env (Vis op i ko)) ≡
+        (Vis op i (laterO_map (λne y, interp_ectx K env y) ◎ ko))).
+      { by rewrite hom_vis. }
+      trans (IF (Vis op i (laterO_map (λne y : IT, interp_ectx K env y) ◎ ko))
+               (interp_expr e1 env) (interp_expr e2 env)).
+      { do 3 f_equiv. by rewrite hom_vis. }
+      rewrite IF_Vis. f_equiv. simpl.
+      intro. simpl. by rewrite -laterO_map_compose.
+    - trans (IF (Err e) (interp_expr e1 env) (interp_expr e2 env)).
+      { repeat f_equiv. apply hom_err. }
+      apply IF_Err.
+  Qed.
+
+  #[global] Instance interp_ectx_hom_appr {S} (K : ectx S)
+    (e : expr S) env :
+    IT_hom (interp_ectx K env) ->
+    IT_hom (interp_ectx (AppRK e K) env).
+  Proof.
+    intros. simple refine (IT_HOM _ _ _ _ _); intros; simpl.
+    - by rewrite !hom_tick.
+    - rewrite !hom_vis. f_equiv. intro x. simpl.
+      by rewrite laterO_map_compose.
+    - by rewrite !hom_err.
+  Qed.
+
+  #[global] Instance interp_ectx_hom_appl {S} (K : ectx S)
+    (v : val S) (env : interp_scope S) :
+    IT_hom (interp_ectx K env) ->
+    IT_hom (interp_ectx (AppLK K v) env).
+  Proof.
+    intros H. simple refine (IT_HOM _ _ _ _ _); intros; simpl.
+    - rewrite -APP'_Tick_l. do 2 f_equiv. apply hom_tick.
+    - trans (APP' (Vis op i (laterO_map (interp_ectx K env) ◎ ko))
+               (interp_val v env)).
+      + do 2f_equiv. rewrite hom_vis. do 3 f_equiv. by intro.
+      + rewrite APP'_Vis_l. f_equiv. intro x. simpl.
+        by rewrite -laterO_map_compose.
+    - trans (APP' (Err e) (interp_val v env)).
+      { do 2f_equiv. apply hom_err. }
+      apply APP'_Err_l, interp_val_asval.
+  Qed.
+
+  #[global] Instance interp_ectx_hom_natopr {S} (K : ectx S)
+    (e : expr S) op env :
+    IT_hom (interp_ectx K env) ->
+    IT_hom (interp_ectx (NatOpRK op e K) env).
+  Proof.
+    intros H. simple refine (IT_HOM _ _ _ _ _); intros; simpl.
+    - by rewrite !hom_tick.
+    - rewrite !hom_vis. f_equiv. intro x. simpl.
+      by rewrite laterO_map_compose.
+    - by rewrite !hom_err.
+  Qed.
+
+  #[global] Instance interp_ectx_hom_natopl {S} (K : ectx S)
+    (v : val S) op (env : interp_scope S) :
+    IT_hom (interp_ectx K env) ->
+    IT_hom (interp_ectx (NatOpLK op K v) env).
+  Proof.
+    intros H. simple refine (IT_HOM _ _ _ _ _); intros; simpl.
+    - rewrite -NATOP_ITV_Tick_l. do 2 f_equiv. apply hom_tick.
+    - trans (NATOP (do_natop op)
+               (Vis op0 i (laterO_map (interp_ectx K env) ◎ ko))
+               (interp_val v env)).
+      { do 2 f_equiv. rewrite hom_vis. f_equiv. by intro. }
+      rewrite NATOP_ITV_Vis_l. f_equiv. intro x. simpl.
+      by rewrite -laterO_map_compose.
+    - trans (NATOP (do_natop op) (Err e) (interp_val v env)).
+      + do 2 f_equiv. apply hom_err.
+      + by apply NATOP_Err_l, interp_val_asval.
+  Qed.
+
+  Lemma get_fun_ret' E A `{Cofe A} n : (∀ f, @get_fun E A _ f (core.Ret n) ≡ Err RuntimeErr).
+  Proof.
+    intros.
+    by rewrite IT_rec1_ret.
+  Qed.
+
+  #[global] Instance interp_ectx_hom {S}
+    (K : ectx S) env :
     IT_hom (interp_ectx K env).
-  Proof. induction K; simpl; apply _. Qed.
+  Proof.
+    induction K; apply _.
+  Qed.
 
   (** ** Finally, preservation of reductions *)
-  Lemma interp_expr_head_step {S} env (e : expr S) e' σ σ' n :
-    head_step e σ e' σ' (n,0) →
+  Lemma interp_expr_head_step {S : Set} (env : interp_scope S) (e : expr S) e' σ σ' n :
+    head_step e σ e' σ' (n, 0) →
     interp_expr e env ≡ Tick_n n $ interp_expr e' env.
   Proof.
     inversion 1; cbn-[IF APP' INPUT Tick get_ret2].
-    - (*fun->val*)
-      reflexivity.
     - (* app lemma *)
-      rewrite APP_APP'_ITV.
+      subst.
+      erewrite APP_APP'_ITV; last apply _.
       trans (APP (Fun (Next (ir_unf (interp_expr e1) env))) (Next $ interp_val v2 env)).
       { repeat f_equiv. apply interp_rec_unfold. }
       rewrite APP_Fun. simpl. rewrite Tick_eq. do 2 f_equiv.
       simplify_eq.
-      rewrite interp_expr_subst. f_equiv.
-      simp interp_subs_scope. unfold hd_sub, tl_sub. simp conssub.
-      simpl. repeat f_equiv.
-      generalize (Val (RecV e1)).
-      generalize (Val v2).
-      clear.
-      intros e1 e2.
-      trans (interp_subs_scope env idsub); last first.
-      {  f_equiv. intro v. simp conssub. done. }
-      symmetry.
-      apply interp_subs_scope_idsub.
+      rewrite !interp_expr_subst.
+      f_equiv.
+      intros [| [| x]]; simpl; [| reflexivity | reflexivity].
+      rewrite interp_val_ren.
+      f_equiv.
+      intros ?; simpl; reflexivity.
     - (* the natop stuff *)
       simplify_eq.
       destruct v1,v2; try naive_solver. simpl in *.
       rewrite NATOP_Ret.
       destruct op; simplify_eq/=; done.
-    - by rewrite IF_True.
-    - rewrite IF_False; eauto. lia.
+    - rewrite IF_True; last lia.
+      reflexivity.
+    - rewrite IF_False; last lia.
+      reflexivity.
   Qed.
 
-  Lemma interp_expr_fill_no_reify {S} K env (e e' : expr S) σ σ' n :
-    head_step e σ e' σ' (n,0) →
-    interp_expr (fill K e) env ≡ Tick_n n $ interp_expr (fill K e') env.
+  Lemma interp_expr_fill_no_reify {S} K (env : interp_scope S) (e e' : expr S) σ σ' n :
+    head_step e σ e' σ' (n, 0) →
+    interp_expr (fill K e) env
+      ≡
+      Tick_n n $ interp_expr (fill K e') env.
   Proof.
     intros He.
-    trans (interp_ectx K env (interp_expr e env)).
-    { apply interp_ectx_fill. }
-    trans (interp_ectx K env (Tick_n n (interp_expr e' env))).
-    {  f_equiv. apply (interp_expr_head_step env) in He. apply He. }
-    trans (Tick_n n $ interp_ectx K env (interp_expr e' env)); last first.
-    { f_equiv. symmetry. apply interp_ectx_fill. }
-    apply hom_tick_n. apply _.
+    rewrite !interp_comp.
+    erewrite <-hom_tick_n.
+    - apply (interp_expr_head_step env) in He.
+      rewrite He.
+      reflexivity.
+    - apply _.
   Qed.
 
   Opaque INPUT OUTPUT_.
+  Opaque extend_scope.
   Opaque Ret.
 
   Lemma interp_expr_fill_yes_reify {S} K env (e e' : expr S)
-    (σ σ' : stateO) (σr : gState_rest sR_idx rs ♯ IT) n :
-    head_step e σ e' σ' (n,1) →
-    reify (gReifiers_sReifier rs)
-      (interp_expr (fill K e) env)  (gState_recomp σr (sR_state σ))
-      ≡ (gState_recomp σr (sR_state σ'), Tick_n n $ interp_expr (fill K e') env).
+    (σ σ' : stateO) (σr : gState_rest NotCtxDep sR_idx rs ♯ IT) n :
+    head_step e σ e' σ' (n, 1) →
+    reify (gReifiers_sReifier NotCtxDep rs)
+      (interp_expr (fill K e) env) (gState_recomp NotCtxDep σr (sR_state σ))
+      ≡ (gState_recomp NotCtxDep σr (sR_state σ'), Tick_n n $ interp_expr (fill K e') env).
   Proof.
     intros Hst.
-    trans (reify (gReifiers_sReifier rs) (interp_ectx K env (interp_expr e env))
-             (gState_recomp σr (sR_state σ))).
-    { f_equiv. by rewrite interp_ectx_fill. }
+    trans (reify (gReifiers_sReifier NotCtxDep rs) (interp_ectx K env (interp_expr e env))
+             (gState_recomp NotCtxDep σr (sR_state σ))).
+    { f_equiv. by rewrite interp_comp. }
     inversion Hst; simplify_eq; cbn-[gState_recomp].
-    - trans (reify (gReifiers_sReifier rs) (INPUT (interp_ectx K env ◎ Ret)) (gState_recomp σr (sR_state σ))).
-      { repeat f_equiv; eauto.
-        rewrite hom_INPUT. f_equiv. by intro. }
-      rewrite reify_vis_eq //; last first.
-      { rewrite subReifier_reify//= H4//=. }
-      repeat f_equiv.
-      rewrite Tick_eq/=. repeat f_equiv.
-      rewrite interp_ectx_fill.
-      simpl.
-      done.
-    - trans (reify (gReifiers_sReifier rs) (interp_ectx K env (OUTPUT n0)) (gState_recomp σr (sR_state σ))).
-      { do 3 f_equiv; eauto.
-        rewrite get_ret_ret//. }
-      trans (reify (gReifiers_sReifier rs) (OUTPUT_ n0 (interp_ectx K env (Ret 0))) (gState_recomp σr (sR_state σ))).
-      { do 2 f_equiv; eauto.
-        rewrite hom_OUTPUT_//. }
-      rewrite reify_vis_eq //; last first.
+    - trans (reify (gReifiers_sReifier NotCtxDep rs) (INPUT (interp_ectx K env ◎ Ret)) (gState_recomp NotCtxDep σr (sR_state σ))).
       {
+        repeat f_equiv; eauto.
+        rewrite hom_INPUT.
+        do 2 f_equiv. by intro.
+      }
+      rewrite reify_vis_eq_ctx_indep //; first last.
+      {
+        epose proof (@subReifier_reify sz NotCtxDep reify_io rs _ IT _ (inl ()) () _ σ σ' σr) as H.
+        simpl in H.
         simpl.
-        pose proof (@subReifier_reify sz reify_io rs subR IT _ ((inr (inl ()))) n0) as H.
-        simpl in H.
-        specialize (H (Next (interp_ectx K env (Ret 0))) (λne _, Next (interp_ectx K env (Ret 0))) σ (update_output n0 σ) σr).
-        simpl in H.
-        rewrite <-H; last done.
-        f_equiv.
-        - intros [? ?] [? ?] [? ?]; simpl in *.
+        erewrite <-H; last first.
+        - rewrite H4. reflexivity.
+        - f_equiv;
           solve_proper.
-        - do 2 f_equiv.
-          intros ?; simpl.
-          reflexivity.
       }
       repeat f_equiv. rewrite Tick_eq/=. repeat f_equiv.
-      rewrite interp_ectx_fill.
-      simpl. done.
+      rewrite interp_comp.
+      rewrite ofe_iso_21.
+      simpl.
+      reflexivity.
+    - trans (reify (gReifiers_sReifier NotCtxDep rs) (interp_ectx K env (OUTPUT n0)) (gState_recomp NotCtxDep σr (sR_state σ))).
+      {
+        do 3 f_equiv; eauto.
+        rewrite get_ret_ret//.
+      }
+      trans (reify (gReifiers_sReifier NotCtxDep rs) (OUTPUT_ n0 (interp_ectx K env (Ret 0))) (gState_recomp NotCtxDep σr (sR_state σ))).
+      {
+        do 2 f_equiv; eauto.
+        by rewrite hom_OUTPUT_.
+      }
+      rewrite reify_vis_eq_ctx_indep //; last first.
+      {
+        epose proof (@subReifier_reify sz NotCtxDep reify_io rs _ IT _ (inr (inl ())) n0 _ σ (update_output n0 σ) σr) as H.
+        simpl in H.
+        simpl.
+        erewrite <-H; last reflexivity.
+        f_equiv.
+        intros ???. by rewrite /prod_map H0.
+      }
+      repeat f_equiv. rewrite Tick_eq/=. repeat f_equiv.
+      rewrite interp_comp.
+      reflexivity.
   Qed.
 
-  Lemma soundness {S} (e1 e2 : expr S) σ1 σ2 (σr : gState_rest sR_idx rs ♯ IT) n m env :
+  Lemma soundness {S} (e1 e2 : expr S) σ1 σ2 (σr : gState_rest NotCtxDep sR_idx rs ♯ IT) n m (env : interp_scope S) :
     prim_step e1 σ1 e2 σ2 (n,m) →
-    ssteps (gReifiers_sReifier rs)
-              (interp_expr e1 env) (gState_recomp σr (sR_state σ1))
-              (interp_expr e2 env) (gState_recomp σr (sR_state σ2)) n.
+    ssteps (gReifiers_sReifier NotCtxDep rs)
+              (interp_expr e1 env) (gState_recomp NotCtxDep σr (sR_state σ1))
+              (interp_expr e2 env) (gState_recomp NotCtxDep σr (sR_state σ2)) n.
   Proof.
     Opaque gState_decomp gState_recomp.
     inversion 1; simplify_eq/=.
     destruct (head_step_io_01 _ _ _ _ _ _ H2); subst.
     - assert (σ1 = σ2) as ->.
       { eapply head_step_no_io; eauto. }
-      eapply (interp_expr_fill_no_reify K) in H2.
-      rewrite H2. eapply ssteps_tick_n.
+      unshelve eapply (interp_expr_fill_no_reify K) in H2; first apply env.
+      rewrite H2.
+      rewrite interp_comp.
+      eapply ssteps_tick_n.
     - inversion H2;subst.
       + eapply (interp_expr_fill_yes_reify K env _ _ _ _ σr) in H2.
-        rewrite interp_ectx_fill.
+        rewrite interp_comp.
         rewrite hom_INPUT.
-        change 1 with (1+0). econstructor; last first.
+        change 1 with (Nat.add 1 0). econstructor; last first.
         { apply ssteps_zero; reflexivity. }
         eapply sstep_reify.
         { Transparent INPUT. unfold INPUT. simpl.
@@ -655,13 +691,13 @@ Section interp.
         simpl in H2.
         rewrite -H2.
         repeat f_equiv; eauto.
-        rewrite interp_ectx_fill hom_INPUT.
+        rewrite interp_comp hom_INPUT.
         eauto.
       + eapply (interp_expr_fill_yes_reify K env _ _ _ _ σr) in H2.
-        rewrite interp_ectx_fill. simpl.
+        rewrite interp_comp. simpl.
         rewrite get_ret_ret.
         rewrite hom_OUTPUT_.
-        change 1 with (1+0). econstructor; last first.
+        change 1 with (Nat.add 1 0). econstructor; last first.
         { apply ssteps_zero; reflexivity. }
         eapply sstep_reify.
         { Transparent OUTPUT_. unfold OUTPUT_. simpl.
@@ -670,7 +706,7 @@ Section interp.
         rewrite -H2.
         repeat f_equiv; eauto.
         Opaque OUTPUT_.
-        rewrite interp_ectx_fill /= get_ret_ret hom_OUTPUT_.
+        rewrite interp_comp /= get_ret_ret hom_OUTPUT_.
         eauto.
   Qed.
 
