theories/input_lang_callcc/hom.v
@@ -1,16 +1,15 @@
-From Equations Require Import Equations.
 From gitrees Require Import gitree.
 From gitrees.input_lang_callcc Require Import lang interp.
-Require Import gitrees.lang_generic_sem.
+Require Import gitrees.lang_generic.
 Require Import Binding.Lib Binding.Set Binding.Env.
 
 Open Scope stdpp_scope.
 
 Section hom.
   Context {sz : nat}.
-  Context {rs : gReifiers sz}.
+  Context {rs : gReifiers CtxDep sz}.
   Context {subR : subReifier reify_io rs}.
-  Notation F := (gReifiers_ops rs).
+  Notation F := (gReifiers_ops CtxDep rs).
   Notation IT := (IT F natO).
   Notation ITV := (ITV F natO).
 
